wip

src/riot/RIoT.Core.fst
@@ -54,6 +54,7 @@ type aliasKeyCRT_ingredients_t = {
   aliasKeyCrt_riot_version: datatype_of_asn1_type INTEGER;
 }
 
+unfold
 let deviceIDCRI_pre (x:deviceIDCSR_ingredients_t) =
   True
   // valid_deviceIDCRI_ingredients
@@ -64,6 +65,7 @@ unfold noextract
 let coerce_asn1_tlv_int32_of_type_to_asn1_int32 (x:asn1_TLV_int32_of_type SEQUENCE)
   : asn1_int32 = x
 
+unfold
 let deviceIDCSR_pre (x:deviceIDCSR_ingredients_t{deviceIDCRI_pre x}) (deviceIDCSR_len:UInt32.t) =
   let l = coerce_asn1_tlv_int32_of_type_to_asn1_int32
     (len_of_deviceIDCRI
@@ -73,6 +75,7 @@ let deviceIDCSR_pre (x:deviceIDCSR_ingredients_t{deviceIDCRI_pre x}) (deviceIDCS
   valid_deviceIDCSR_ingredients l /\
   eq2 #nat (v deviceIDCSR_len) (length_of_deviceIDCSR l)
 
+unfold
 let aliasKeyCRT_pre (x:aliasKeyCRT_ingredients_t) (aliasKeyCRT_len:UInt32.t) =
   let l = coerce_asn1_tlv_int32_of_type_to_asn1_int32
     (len_of_aliasKeyTBS
@@ -82,6 +85,7 @@ let aliasKeyCRT_pre (x:aliasKeyCRT_ingredients_t) (aliasKeyCRT_len:UInt32.t) =
   valid_aliasKeyCRT_ingredients l /\
   eq2 #nat (v aliasKeyCRT_len) (length_of_aliasKeyCRT l)
 
+unfold
 let riot_pre
   (h: HS.mem)
 (* Common Inputs *)
@@ -129,6 +133,7 @@ let riot_pre
    deviceIDCSR_pre deviceIDCSR_ingredients deviceIDCSR_len /\
    aliasKeyCRT_pre aliasKeyCRT_ingredients aliasKeyCRT_len
 
+unfold
 let aliasKey_post
   (cdi : B.lbuffer byte_sec 32) (fwid: B.lbuffer byte_sec 32)
   (aliasKey_label_len:UInt32.t{valid_hkdf_lbl_len aliasKey_label_len})
@@ -144,6 +149,7 @@ let aliasKey_post
                                                        (B.as_seq h0 aliasKey_label)
 
 #push-options "--z3rlimit 100"
+unfold
 let deviceIDCSR_post
   (cdi:B.lbuffer byte_sec 32)
   (deviceID_label_len:UInt32.t{valid_hkdf_lbl_len deviceID_label_len})
@@ -164,12 +170,12 @@ let deviceIDCSR_post
       deviceIDCSR_ingredients.deviceIDCSR_ku deviceID_pub_seq in
 
     let deviceIDCRI_seq = serialize_deviceIDCRI `serialize` deviceIDCRI in
-    
+
     let deviceIDCRI_len = coerce_asn1_tlv_int32_of_type_to_asn1_int32
       (len_of_deviceIDCRI
         deviceIDCSR_ingredients.deviceIDCSR_version deviceIDCSR_ingredients.deviceIDCSR_s_common
         deviceIDCSR_ingredients.deviceIDCSR_s_org deviceIDCSR_ingredients.deviceIDCSR_s_country) in
-      
+
     let (* Prf *) _ = lemma_serialize_deviceIDCRI_size_exact deviceIDCRI in  //AR: TODO: This takes long time
     let deviceIDCSR: deviceIDCSR_t deviceIDCRI_len = sign_and_finalize_deviceIDCSR_spec
                                                                 (deviceID_priv_seq)
@@ -182,6 +188,7 @@ unfold noextract
 let coerce_asn1_int32_to_size_t (x:asn1_int32) : size_t = x
 
 #push-options "--z3rlimit 100"
+unfold
 let aliasKeyCRT_post
   (cdi:B.lbuffer byte_sec 32)
   (fwid: B.lbuffer byte_sec 32)
@@ -228,14 +235,14 @@ let aliasKeyCRT_post
          aliasKeyCRT_ingredients.aliasKeyCrt_s_country
          aliasKeyCRT_ingredients.aliasKeyCrt_riot_version) in
      let (* Prf *) _ = lemma_serialize_aliasKeyTBS_size_exact aliasKeyTBS in
-     assume (Seq.length aliasKeyTBS_seq == v aliasKeyTBS_len); //TODO: help Z3 prove it
+     assert (Seq.length aliasKeyTBS_seq == v aliasKeyTBS_len); //TODO: help Z3 prove it
      let aliasKeyCRT: aliasKeyCRT_t aliasKeyTBS_len = sign_and_finalize_aliasKeyCRT_spec
                                                                 (deviceID_priv_seq)
                                                                 (aliasKeyTBS_len)
                                                                 (aliasKeyTBS_seq) in
      B.as_seq h1 aliasKeyCRT_buf == serialize_aliasKeyCRT aliasKeyTBS_len `serialize` aliasKeyCRT
 
-
+unfold
 let riot_post
 (* Common Inputs *)
   (cdi : B.lbuffer byte_sec 32)
@@ -263,24 +270,312 @@ let riot_post
     aliasKeyCRT_ingredients aliasKey_pub aliasKey_priv
     deviceIDCSR_len deviceIDCSR_buf
     aliasKeyCRT_len aliasKeyCRT_buf})
-  (h1:HS.mem) 
+  (h1:HS.mem)
   : Type0
   =
-    // B.(modifies (loc_buffer deviceIDCSR_buf `loc_union`
-    //              loc_buffer aliasKeyCRT_buf `loc_union`
-    //              loc_buffer aliasKey_pub    `loc_union`
-    //              loc_buffer aliasKey_priv ) h0 h1) /\
+    B.(modifies (loc_buffer aliasKey_pub    `loc_union`
+                 loc_buffer aliasKey_priv   `loc_union`
+                 loc_buffer deviceIDCSR_buf `loc_union`
+                 loc_buffer aliasKeyCRT_buf
+                 ) h0 h1) /\
 
-    // aliasKey_post cdi fwid aliasKey_label_len aliasKey_label aliasKey_pub aliasKey_priv h0 h1 /\
-    
+    aliasKey_post cdi fwid aliasKey_label_len aliasKey_label aliasKey_pub aliasKey_priv h0 h1 /\
+
     // deviceIDCSR_post cdi deviceID_label_len deviceID_label
     //   deviceIDCSR_ingredients deviceIDCSR_len deviceIDCSR_buf h0 h1 /\
-    
+
     // aliasKeyCRT_post cdi fwid deviceID_label_len deviceID_label
     //   aliasKeyCRT_ingredients aliasKeyCRT_len aliasKeyCRT_buf aliasKey_pub h0 h1 /\
 True
 
-// #set-options "--z3rlimit 256"
+let () = ()
+// let f ()
+// : HST.St unit
+// = let h0 = HST.get () in
+//   HST.push_frame ();
+//   HST.pop_frame ();
+//   let h1 = HST.get () in
+//   assert (HST.equal_domains h0 h1)
+
+module U32 = FStar.UInt32
+module U8 = FStar.UInt8
+#reset-options
+
+let lemma_help
+  (pub_t sec_t: Type0)
+  (h0 hs0 hsf hf: HS.mem)
+  (in1: B.buffer sec_t) (in2: B.buffer sec_t) (in3: B.buffer sec_t) (in4: B.buffer sec_t)
+  (out1: B.buffer pub_t) (out2: B.buffer sec_t) (out3: B.buffer pub_t) (out4: B.buffer pub_t)
+  (hs1 hs2 hs3 hs4 hs5 hs6 hs7 hs8 hs9 hs10 hs11 hs12 hs13 hs14: HS.mem)
+  (_bl1: UInt32.t) (_b1: B.lbuffer pub_t (U32.v _bl1)) (_bv1: pub_t)
+  (_bl2: UInt32.t) (_b2: B.lbuffer sec_t (U32.v _bl2)) (_bv2: sec_t)
+  (_bl3: UInt32.t) (_b3: B.lbuffer sec_t (U32.v _bl3)) (_bv3: sec_t)
+  (_bl4: UInt32.t) (_b4: B.lbuffer pub_t (U32.v _bl4)) (_bv4: pub_t)
+  (_bl5: UInt32.t) (_b5: B.lbuffer pub_t (U32.v _bl5)) (_bv5: pub_t)
+  (_bl6: UInt32.t) (_b6: B.lbuffer pub_t (U32.v _bl6)) (_bv6: pub_t)
+: Lemma
+  (requires
+            B.all_live h0 [B.buf in1; B.buf in2; B.buf in3; B.buf in4;
+                           B.buf out1; B.buf out2; B.buf out3; B.buf out4] /\
+            B.all_disjoint [B.loc_buffer in1; B.loc_buffer in2; B.loc_buffer in3; B.loc_buffer in4;
+                            B.loc_buffer out1; B.loc_buffer out2; B.loc_buffer out3; B.loc_buffer out4] /\
+            HS.fresh_frame h0 hs0 /\ HS.get_tip hs0 == HS.get_tip hsf /\ HS.popped hsf hf /\
+            B.alloc_post_mem_common _b1 hs0 hs1 (Seq.create (UInt32.v _bl1) _bv1) /\ B.frameOf _b1 == HS.get_tip hs0 /\
+            B.alloc_post_mem_common _b2 hs1 hs2 (Seq.create (UInt32.v _bl2) _bv2) /\ B.frameOf _b2 == HS.get_tip hs1 /\
+            B.alloc_post_mem_common _b3 hs2 hs3 (Seq.create (UInt32.v _bl3) _bv3) /\ B.frameOf _b3 == HS.get_tip hs2 /\
+            B.alloc_post_mem_common _b4 hs3 hs4 (Seq.create (UInt32.v _bl4) _bv4) /\ B.frameOf _b4 == HS.get_tip hs3 /\
+
+            (* Derive DeviceID *)
+            B.modifies (B.loc_buffer _b1 `B.loc_union` B.loc_buffer _b2) hs4 hs5 /\
+
+            (* Derive AliasKey *)
+            B.modifies (B.loc_buffer out1 `B.loc_union` B.loc_buffer out2) hs5 hs6 /\
+
+            (* Classify DeviceID Public Key *)
+            B.modifies (B.loc_buffer _b3) hs6 hs7 /\
+
+            (* Derive AliasCRT_AuthKeyID *)
+            B.modifies (B.loc_buffer _b4) hs7 hs8 /\
+
+            (* Allocate `deviceIDCRI_buf` *)
+            B.alloc_post_mem_common _b5 hs8 hs9 (Seq.create (UInt32.v _bl5) _bv5) /\ B.frameOf _b5 == HS.get_tip hs8 /\
+
+            (* Write `deviceIDCRI_buf` *)
+            B.modifies (B.loc_buffer _b5) hs9 hs10 /\
+
+            (* Write `deviceIDCSR_buf` *)
+            B.modifies (B.loc_buffer out3) hs10 hs11 /\
+
+            (* Allocate `aliasKeyTBS_buf` *)
+            B.alloc_post_mem_common _b6 hs11 hs12 (Seq.create (UInt32.v _bl6) _bv6) /\ B.frameOf _b6 == HS.get_tip hs11 /\
+
+            (* Write `aliasKeyTBS_buf` *)
+            B.modifies (B.loc_buffer _b6) hs12 hs13 /\
+
+            (* Write `aliasKeyCRT_buf` *)
+            B.modifies (B.loc_buffer out4) hs13 hs14 /\
+
+            hs14 == hsf
+            )
+  (ensures
+    B.modifies (B.loc_buffer out1 `B.loc_union`
+                B.loc_buffer out2 `B.loc_union`
+                B.loc_buffer out3 `B.loc_union`
+                B.loc_buffer out4) h0 hf /\
+
+    B.as_seq hs4  in1  == B.as_seq h0 in1 /\ // cdi
+    B.as_seq hs4  in3  == B.as_seq h0 in3 /\ // lbl device
+
+    B.as_seq hs5  in1  == B.as_seq h0 in1 /\ // cdi
+    B.as_seq hs5  in2  == B.as_seq h0 in2 /\ // fwid
+    B.as_seq hs5  in4  == B.as_seq h0 in4 /\ // lbl alias
+
+    B.as_seq hs6  out1 == B.as_seq hf out1 /\
+    B.as_seq hs6  out2 == B.as_seq hf out2 /\
+    B.as_seq hs11 out3 == B.as_seq hf out3 /\
+    B.as_seq hs14 out4 == B.as_seq hf out4 /\
+    True
+  )
+=
+  B.modifies_trans B.loc_none h0 hs0 B.loc_none hs1;
+  B.modifies_trans B.loc_none h0 hs1 B.loc_none hs2;
+  B.modifies_trans B.loc_none h0 hs2 B.loc_none hs3;
+  B.modifies_trans B.loc_none h0 hs3 B.loc_none hs4;
+
+  B.modifies_buffer_elim in1 B.loc_none h0 hs4;
+  B.modifies_buffer_elim in3 B.loc_none h0 hs4;
+
+(* hs4 --> hs5 *)
+  B.modifies_trans B.loc_none h0 hs4 (
+    B.loc_buffer _b1 `B.loc_union`
+    B.loc_buffer _b2
+  ) hs5;
+  B.modifies_buffer_elim in1 (B.loc_buffer out1 `B.loc_union` B.loc_buffer out2) h0 hs5;
+  B.modifies_buffer_elim in2 (B.loc_buffer out1 `B.loc_union` B.loc_buffer out2) h0 hs5;
+  B.modifies_buffer_elim in4 (B.loc_buffer out1 `B.loc_union` B.loc_buffer out2) h0 hs5;
+
+(* hs5 --> hs6 *)
+  B.modifies_trans (
+    B.loc_buffer _b1 `B.loc_union`
+    B.loc_buffer _b2
+  ) h0 hs5 (
+    B.loc_buffer out1 `B.loc_union`
+    B.loc_buffer out2
+  ) hs6;
+  B.modifies_buffer_elim _b1 (B.loc_buffer out1 `B.loc_union` B.loc_buffer out2) hs5 hs6;
+  B.modifies_buffer_elim _b2 (B.loc_buffer out1 `B.loc_union` B.loc_buffer out2) hs5 hs6;
+
+(* hs6 --> hs7 *)
+  B.modifies_trans (
+    B.loc_buffer _b1 `B.loc_union`
+    B.loc_buffer _b2 `B.loc_union`
+    B.loc_buffer out1  `B.loc_union`
+    B.loc_buffer out2
+  ) h0 hs6 (
+    B.loc_buffer _b3
+  ) hs7;
+  B.modifies_buffer_elim _b1 (B.loc_buffer _b3) hs6 hs7;
+  B.modifies_buffer_elim _b2 (B.loc_buffer _b3) hs6 hs7;
+  B.modifies_buffer_elim out1  (B.loc_buffer _b3) hs6 hs7;
+  B.modifies_buffer_elim out2  (B.loc_buffer _b3) hs6 hs7;
+
+(* hs7 --> hs8 *)
+  B.modifies_trans (
+    B.loc_buffer _b1 `B.loc_union`
+    B.loc_buffer _b2 `B.loc_union`
+    B.loc_buffer out1  `B.loc_union`
+    B.loc_buffer out2  `B.loc_union`
+    B.loc_buffer _b3
+  ) h0 hs7 (
+    B.loc_buffer _b4
+  ) hs8;
+  B.modifies_buffer_elim _b1 (B.loc_buffer _b4) hs7 hs8;
+  B.modifies_buffer_elim _b2 (B.loc_buffer _b4) hs7 hs8;
+  B.modifies_buffer_elim out1  (B.loc_buffer _b4) hs7 hs8;
+  B.modifies_buffer_elim out2  (B.loc_buffer _b4) hs7 hs8;
+  B.modifies_buffer_elim _b3 (B.loc_buffer _b4) hs7 hs8;
+
+(* hs8 --> hs9 *)
+  B.modifies_trans (
+    B.loc_buffer _b1 `B.loc_union`
+    B.loc_buffer _b2 `B.loc_union`
+    B.loc_buffer out1  `B.loc_union`
+    B.loc_buffer out2  `B.loc_union`
+    B.loc_buffer _b3 `B.loc_union`
+    B.loc_buffer _b4
+  ) h0 hs8 B.loc_none hs9;
+  B.modifies_buffer_elim _b1 B.loc_none hs8 hs9;
+  B.modifies_buffer_elim _b2 B.loc_none hs8 hs9;
+  B.modifies_buffer_elim out1  B.loc_none hs8 hs9;
+  B.modifies_buffer_elim out2  B.loc_none hs8 hs9;
+  B.modifies_buffer_elim _b3 B.loc_none hs8 hs9;
+  B.modifies_buffer_elim _b4 B.loc_none hs8 hs9;
+
+(* hs9 --> hs10 *)
+  B.modifies_trans (
+    B.loc_buffer _b1 `B.loc_union`
+    B.loc_buffer _b2 `B.loc_union`
+    B.loc_buffer out1  `B.loc_union`
+    B.loc_buffer out2  `B.loc_union`
+    B.loc_buffer _b3 `B.loc_union`
+    B.loc_buffer _b4
+  ) h0 hs9 (
+    B.loc_buffer _b5
+  ) hs10;
+  B.modifies_buffer_elim _b1 (B.loc_buffer _b5) hs9 hs10;
+  B.modifies_buffer_elim _b2 (B.loc_buffer _b5) hs9 hs10;
+  B.modifies_buffer_elim out1  (B.loc_buffer _b5) hs9 hs10;
+  B.modifies_buffer_elim out2  (B.loc_buffer _b5) hs9 hs10;
+  B.modifies_buffer_elim _b3 (B.loc_buffer _b5) hs9 hs10;
+  B.modifies_buffer_elim _b4 (B.loc_buffer _b5) hs9 hs10;
+
+
+(* hs10 --> hs11 *)
+  B.modifies_trans (
+    B.loc_buffer _b1 `B.loc_union`
+    B.loc_buffer _b2 `B.loc_union`
+    B.loc_buffer out1  `B.loc_union`
+    B.loc_buffer out2  `B.loc_union`
+    B.loc_buffer _b3 `B.loc_union`
+    B.loc_buffer _b4 `B.loc_union`
+    B.loc_buffer _b5
+  ) h0 hs10 (
+    B.loc_buffer out3
+  ) hs11;
+  B.modifies_buffer_elim _b1 (B.loc_buffer out3) hs10 hs11;
+  B.modifies_buffer_elim _b2 (B.loc_buffer out3) hs10 hs11;
+  B.modifies_buffer_elim out1  (B.loc_buffer out3) hs10 hs11;
+  B.modifies_buffer_elim out2  (B.loc_buffer out3) hs10 hs11;
+  B.modifies_buffer_elim _b3 (B.loc_buffer out3) hs10 hs11;
+  B.modifies_buffer_elim _b4 (B.loc_buffer out3) hs10 hs11;
+  B.modifies_buffer_elim _b5 (B.loc_buffer out3) hs10 hs11;
+
+(* hs11 --> hs12 *)
+  B.modifies_trans (
+    B.loc_buffer _b1 `B.loc_union`
+    B.loc_buffer _b2 `B.loc_union`
+    B.loc_buffer out1  `B.loc_union`
+    B.loc_buffer out2  `B.loc_union`
+    B.loc_buffer _b3 `B.loc_union`
+    B.loc_buffer _b4 `B.loc_union`
+    B.loc_buffer _b5 `B.loc_union`
+    B.loc_buffer out3
+  ) h0 hs11 B.loc_none hs12;
+  B.modifies_buffer_elim _b1 B.loc_none hs11 hs12;
+  B.modifies_buffer_elim _b2 B.loc_none hs11 hs12;
+  B.modifies_buffer_elim out1  B.loc_none hs11 hs12;
+  B.modifies_buffer_elim out2  B.loc_none hs11 hs12;
+  B.modifies_buffer_elim _b3 B.loc_none hs11 hs12;
+  B.modifies_buffer_elim _b4 B.loc_none hs11 hs12;
+  B.modifies_buffer_elim _b5 B.loc_none hs11 hs12;
+  B.modifies_buffer_elim out3  B.loc_none hs11 hs12;
+
+(* hs12 --> hs13 *)
+  B.modifies_trans (
+    B.loc_buffer _b1 `B.loc_union`
+    B.loc_buffer _b2 `B.loc_union`
+    B.loc_buffer out1  `B.loc_union`
+    B.loc_buffer out2  `B.loc_union`
+    B.loc_buffer _b3 `B.loc_union`
+    B.loc_buffer _b4 `B.loc_union`
+    B.loc_buffer _b5 `B.loc_union`
+    B.loc_buffer out3
+  ) h0 hs12 (
+    B.loc_buffer _b6
+  ) hs13;
+  B.modifies_buffer_elim _b1 (B.loc_buffer _b6) hs12 hs13;
+  B.modifies_buffer_elim _b2 (B.loc_buffer _b6) hs12 hs13;
+  B.modifies_buffer_elim out1  (B.loc_buffer _b6) hs12 hs13;
+  B.modifies_buffer_elim out2  (B.loc_buffer _b6) hs12 hs13;
+  B.modifies_buffer_elim _b3 (B.loc_buffer _b6) hs12 hs13;
+  B.modifies_buffer_elim _b4 (B.loc_buffer _b6) hs12 hs13;
+  B.modifies_buffer_elim _b5 (B.loc_buffer _b6) hs12 hs13;
+  B.modifies_buffer_elim out3  (B.loc_buffer _b6) hs12 hs13;
+
+(* hs13 --> hs14 *)
+  B.modifies_trans (
+    B.loc_buffer _b1 `B.loc_union`
+    B.loc_buffer _b2 `B.loc_union`
+    B.loc_buffer out1  `B.loc_union`
+    B.loc_buffer out2  `B.loc_union`
+    B.loc_buffer _b3 `B.loc_union`
+    B.loc_buffer _b4 `B.loc_union`
+    B.loc_buffer _b5 `B.loc_union`
+    B.loc_buffer out3  `B.loc_union`
+    B.loc_buffer _b6
+  ) h0 hs13 (
+    B.loc_buffer out4
+  ) hs14;
+  B.modifies_buffer_elim _b1 (B.loc_buffer out4) hs13 hs14;
+  B.modifies_buffer_elim _b2 (B.loc_buffer out4) hs13 hs14;
+  B.modifies_buffer_elim out1  (B.loc_buffer out4) hs13 hs14;
+  B.modifies_buffer_elim out2  (B.loc_buffer out4) hs13 hs14;
+  B.modifies_buffer_elim _b3 (B.loc_buffer out4) hs13 hs14;
+  B.modifies_buffer_elim _b4 (B.loc_buffer out4) hs13 hs14;
+  B.modifies_buffer_elim _b5 (B.loc_buffer out4) hs13 hs14;
+  B.modifies_buffer_elim out3  (B.loc_buffer out4) hs13 hs14;
+  B.modifies_buffer_elim _b6 (B.loc_buffer out4) hs13 hs14;
+
+(* FIXME: This can be proved with 256-512 z3rlimits *)
+  assume (B.modifies ((B.loc_all_regions_from false (HS.get_tip hs0)) `B.loc_union`
+                      (B.loc_buffer out1 `B.loc_union`
+                       B.loc_buffer out2 `B.loc_union`
+                       B.loc_buffer out3 `B.loc_union`
+                       B.loc_buffer out4)) hs0 hsf);
+
+  B.modifies_fresh_frame_popped h0 hs0 (
+    B.loc_buffer out1 `B.loc_union`
+    B.loc_buffer out2 `B.loc_union`
+    B.loc_buffer out3 `B.loc_union`
+    B.loc_buffer out4
+  ) hsf hf;
+
+()
+
+let () = ()
+
+#restart-solver
+#set-options "--z3rlimit 50 --fuel 0 --ifuel 0"
 let riot
 (* Common Inputs *)
   (cdi : B.lbuffer byte_sec 32)
@@ -303,10 +598,9 @@ let riot
   (aliasKeyCRT_len: size_t)
   (aliasKeyCRT_buf: B.lbuffer byte_pub (v aliasKeyCRT_len))
 : HST.Stack unit
-  (requires fun h -> riot_pre
-                        (h)
-                        (cdi)
-                        (fwid)
+  (requires fun h ->
+                  riot_pre
+                        (h) (cdi) (fwid)
                         (deviceID_label_len) (deviceID_label)
                         (aliasKey_label_len) (aliasKey_label)
                         (deviceIDCSR_ingredients)
@@ -315,9 +609,9 @@ let riot
                         (deviceIDCSR_len) (deviceIDCSR_buf)
                         (aliasKeyCRT_len) (aliasKeyCRT_buf)
    )
-   (ensures fun h0 _ h1 -> riot_post
-                        (cdi)
-                        (fwid)
+   (ensures fun h0 _ h1 ->
+                        riot_post
+                        (cdi) (fwid)
                         (deviceID_label_len) (deviceID_label)
                         (aliasKey_label_len) (aliasKey_label)
                         (deviceIDCSR_ingredients)
@@ -325,12 +619,35 @@ let riot
                         (aliasKey_pub) (aliasKey_priv)
                         (deviceIDCSR_len) (deviceIDCSR_buf)
                         (aliasKeyCRT_len) (aliasKeyCRT_buf)
-                        (h0) (h1))
-= HST.push_frame ();
+                        (h0) (h1)
+  )
+= (**) let h0 = HST.get () in
+  HST.push_frame ();
+  (**) let hs0 = HST.get () in
+  (**) B.fresh_frame_modifies h0 hs0;
+  // (**) B.modifies_buffer_elim cdi B.loc_none h0 hs0;
+
 
 (* Derive DeviceID *)
   let deviceID_pub : B.lbuffer byte_pub 32 = B.alloca 0x00uy    32ul in
+  let hs1 = HST.get () in
   let deviceID_priv: B.lbuffer byte_sec 32 = B.alloca (u8 0x00) 32ul in
+  let hs2 = HST.get () in
+  let deviceID_pub_sec: B.lbuffer byte_sec 32 = B.alloca (u8 0x00) 32ul in
+  let hs3 = HST.get () in
+  let aliasKeyCrt_keyID: B.lbuffer byte_pub 20 = B.alloca 0x00uy 20ul in
+  let hs4 = HST.get () in
+
+  assume (
+    B.(all_live hs4 [buf deviceID_pub;
+                     buf deviceID_priv;
+                     buf cdi;
+                     buf deviceID_label]) /\
+    B.(all_disjoint [loc_buffer deviceID_pub;
+                     loc_buffer deviceID_priv;
+                     loc_buffer cdi;
+                     loc_buffer deviceID_label])
+  );
   printf "Deriving DeviceID\n" done;
   derive_DeviceID
     (* pub *) deviceID_pub
@@ -338,15 +655,20 @@ let riot
     (* cdi *) cdi
     (* lbl *) deviceID_label_len
               deviceID_label;
+(* hs5 *) let hs5 = HST.get () in
 
-(* A workaround to derive authKeyID for now *)
-  let deviceID_pub_sec: B.lbuffer byte_sec 32 = B.alloca (u8 0x00) 32ul in
-  let aliasKeyCrt_keyID: B.lbuffer byte_pub 20 = B.alloca 0x00uy 20ul in
-  classify_public_buffer 32ul deviceID_pub deviceID_pub_sec;
-  derive_authKeyID aliasKeyCrt_keyID deviceID_pub_sec;
-  // let aliasKeyCrt_keyID: datatype_of_asn1_type OCTET_STRING = (|20ul, B32.of_buffer 20ul aliasKeyCrt_keyID_buf|) in
-
-(* Derive AliasKey *)
+  assume (
+    B.(all_live hs5 [buf aliasKey_pub;
+                     buf aliasKey_priv;
+                     buf cdi;
+                     buf fwid;
+                     buf aliasKey_label]) /\
+    B.(all_disjoint [loc_buffer aliasKey_pub;
+                     loc_buffer aliasKey_priv;
+                     loc_buffer cdi;
+                     loc_buffer fwid;
+                     loc_buffer aliasKey_label])
+  );
   printf "Deriving AliasKey\n" done;
   derive_AliasKey
     (* pub *) aliasKey_pub
@@ -355,6 +677,29 @@ let riot
     (* fwid*) fwid
     (* lbl *) aliasKey_label_len
               aliasKey_label;
+(* hs6 *) let hs6 = HST.get () in
+
+  assert ( aliasKey_post cdi fwid aliasKey_label_len aliasKey_label aliasKey_pub aliasKey_priv hs5 hs6 );
+  // assume ( B.as_seq hs5 cdi == B.as_seq h0 cdi /\
+  //          B.as_seq hs5 fwid == B.as_seq h0 fwid /\
+  //          B.as_seq hs5 aliasKey_label == B.as_seq h0 aliasKey_label);
+  // assert ( aliasKey_post cdi fwid aliasKey_label_len aliasKey_label aliasKey_pub aliasKey_priv h0 hs6 );
+
+  assume (
+    B.live hs6 deviceID_pub /\ B.live hs6 deviceID_pub_sec /\
+    B.disjoint deviceID_pub deviceID_pub_sec
+  );
+  classify_public_buffer 32ul deviceID_pub deviceID_pub_sec;
+(* hs7 *) let hs7 = HST.get () in
+
+  assume (
+    B.live hs7 aliasKeyCrt_keyID /\ B.live hs7 deviceID_pub_sec /\
+    B.disjoint aliasKeyCrt_keyID deviceID_pub_sec
+  );
+  derive_authKeyID
+    aliasKeyCrt_keyID
+    deviceID_pub_sec;
+(* hs8 *) let hs8 = HST.get () in
 
 (* Create DeviceIDCRI *)
    let deviceIDCRI_len: asn1_TLV_int32_of_type SEQUENCE = len_of_deviceIDCRI
@@ -363,7 +708,12 @@ let riot
                                                             deviceIDCSR_ingredients.deviceIDCSR_s_org
                                                             deviceIDCSR_ingredients.deviceIDCSR_s_country in
    let deviceIDCRI_buf: B.lbuffer byte_pub (v deviceIDCRI_len) = B.alloca 0x00uy deviceIDCRI_len in
+(* hs9 *) let hs9 = HST.get () in
 
+   assume (B.(all_live hs9 [buf deviceID_pub;
+                            buf deviceIDCRI_buf]));
+   assume (B.(all_disjoint [loc_buffer deviceID_pub;
+                            loc_buffer deviceIDCRI_buf]));
    printf "Creating DeviceID Certificate Signing Request Information\n" done;
    create_deviceIDCRI
     (* version   *) deviceIDCSR_ingredients.deviceIDCSR_version
@@ -374,8 +724,14 @@ let riot
     (* DeviceID  *) deviceID_pub
     (*DeviceIDCRI*) deviceIDCRI_len
                     deviceIDCRI_buf;
+(* hs10 *) let hs10 = HST.get () in
 
-(* Sign AliasKeyTBS and Finalize AliasKeyCRT *)
+  assume (B.(all_live hs10 [buf deviceID_priv;
+                            buf deviceIDCRI_buf;
+                            buf deviceIDCSR_buf]));
+  assume (B.(all_disjoint [loc_buffer deviceID_priv;
+                           loc_buffer deviceIDCRI_buf;
+                           loc_buffer deviceIDCSR_buf]));
   printf "Signing and finalizing DeviceID Certificate Signing Request\n" done;
   sign_and_finalize_deviceIDCSR
     (*Signing Key*) deviceID_priv
@@ -383,6 +739,8 @@ let riot
                     deviceIDCRI_buf
     (*DeviceIDCSR*) deviceIDCSR_len
                     deviceIDCSR_buf;
+(* hs11 *) let hs11 = HST.get () in
+
 (* Create AliasKeyTBS *)
   let aliasKeyTBS_len: asn1_TLV_int32_of_type SEQUENCE = len_of_aliasKeyTBS
                                                            aliasKeyCRT_ingredients.aliasKeyCrt_serialNumber
@@ -394,6 +752,18 @@ let riot
                                                            aliasKeyCRT_ingredients.aliasKeyCrt_s_country
                                                            aliasKeyCRT_ingredients.aliasKeyCrt_riot_version in
   let aliasKeyTBS_buf: B.lbuffer byte_pub (v aliasKeyTBS_len) = B.alloca 0x00uy aliasKeyTBS_len in
+
+(* hs12 *) let hs12 = HST.get () in
+  assume (B.(all_live hs12 [buf fwid;
+                            buf deviceID_pub;
+                            buf aliasKey_pub;
+                            buf aliasKeyCrt_keyID;
+                            buf aliasKeyTBS_buf]));
+  assume (B.(all_disjoint [loc_buffer fwid;
+                           loc_buffer deviceID_pub;
+                           loc_buffer aliasKey_pub;
+                           loc_buffer aliasKeyCrt_keyID;
+                           loc_buffer aliasKeyTBS_buf]));
 
   printf "Creating AliasKey Certificate TBS\n" done;
   create_aliasKeyTBS
@@ -416,6 +786,14 @@ let riot
     (*AliasKeyTBS*) aliasKeyTBS_len
                     aliasKeyTBS_buf;
 
+(* hs13 *) let hs13 = HST.get () in
+  assume (B.(all_live hs13 [buf deviceID_priv;
+                            buf aliasKeyTBS_buf;
+                            buf aliasKeyCRT_buf]));
+  assume (B.(all_disjoint [loc_buffer deviceID_priv;
+                           loc_buffer aliasKeyTBS_buf;
+                           loc_buffer aliasKeyCRT_buf]));
+
 (* Sign AliasKeyTBS and Finalize AliasKeyCRT *)
   printf "Signing and finalizing AliasKey Certificate\n" done;
   sign_and_finalize_aliasKeyCRT
@@ -425,4 +803,321 @@ let riot
     (*AliasKeyCRT*) aliasKeyCRT_len
                     aliasKeyCRT_buf;
 
-  HST.pop_frame()
+(* hs14 *) let hs14 = HST.get () in
+
+(* hsf *) let hsf = HST.get () in
+  HST.pop_frame ();
+(* hf *) let hf = HST.get () in
+  (**) B.popped_modifies hsf hf;
+
+  lemma_help
+    byte_pub byte_sec
+    h0 hs0 hsf hf
+    cdi fwid deviceID_label aliasKey_label
+    aliasKey_pub aliasKey_priv deviceIDCSR_buf aliasKeyCRT_buf
+    hs1 hs2 hs3 hs4 hs5 hs6 hs7 hs8 hs9 hs10 hs11 hs12 hs13 hs14
+    32ul deviceID_pub 0x00uy
+    32ul deviceID_priv (u8 0x00)
+    32ul deviceID_pub_sec (u8 0x00)
+    20ul aliasKeyCrt_keyID 0x00uy
+    deviceIDCRI_len deviceIDCRI_buf 0x00uy
+    aliasKeyTBS_len aliasKeyTBS_buf 0x00uy;
+
+  assert ( B.as_seq hs5 cdi == B.as_seq h0 cdi /\
+           B.as_seq hs5 fwid == B.as_seq h0 fwid /\
+           B.as_seq hs5 aliasKey_label == B.as_seq h0 aliasKey_label);
+  assert ( aliasKey_post cdi fwid aliasKey_label_len aliasKey_label aliasKey_pub aliasKey_priv h0 hs6 );
+  assert ( B.as_seq hs6 aliasKey_pub  == B.as_seq hf aliasKey_pub /\
+           B.as_seq hs6 aliasKey_priv == B.as_seq hf aliasKey_priv );
+  assert ( aliasKey_post cdi fwid aliasKey_label_len aliasKey_label aliasKey_pub aliasKey_priv h0 hf );
+
+  assume (HST.equal_domains h0 hf)
+
+
+(*
+
+
+
+  // assert (HS.fresh_frame h0 hs0 /\ HS.get_tip hs0 == HS.get_tip hsf /\ HS.popped hsf hf);
+  // let _b1, _bv1, _bl1 = deviceID_pub, 0x00uy, 32ul in
+  // assert (B.alloc_post_mem_common _b1 hs0 hs1 (Seq.create (UInt32.v _bl1) _bv1) /\ B.frameOf _b1 == HS.get_tip hs0);
+  // let _b2, _bv2, _bl2 = deviceID_priv, (u8 0x00), 32ul in
+  // assert (B.alloc_post_mem_common _b2 hs1 hs2 (Seq.create (UInt32.v _bl2) _bv2) /\ B.frameOf _b2 == HS.get_tip hs1);
+  // let _b3, _bv3, _bl3 = deviceID_pub_sec, (u8 0x00), 32ul in
+  // assert (B.alloc_post_mem_common _b3 hs2 hs3 (Seq.create (UInt32.v _bl3) _bv3) /\ B.frameOf _b3 == HS.get_tip hs2);
+  // let _b4, _bv4, _bl4 = aliasKeyCrt_keyID, 0x00uy, 20ul in
+  // assert (B.alloc_post_mem_common _b4 hs3 hs4 (Seq.create (UInt32.v _bl4) _bv4) /\ B.frameOf _b4 == HS.get_tip hs3);
+  // assert (hs4 == hsf);
+  // let _b5, _bv5, _bl5 = deviceIDCRI_buf, 0x00uy, deviceIDCRI_len in
+  // assert (B.modifies (B.loc_buffer _b5) hs9 hs10); admit();
+
+  (**) let hs1 = HST.get () in
+  (**) B.modifies_trans B.loc_none h0 hs0 B.loc_none hs1;
+  // (**) B.modifies_buffer_elim cdi B.loc_none h0 hs1;
+  // (**) assume (B.(all_live hs1 [buf deviceID_pub;
+  //                               buf deviceID_priv;
+  //                               buf cdi;
+  //                               buf deviceID_label]));
+  // assume (B.(all_disjoint [loc_buffer deviceID_pub;
+  //                          loc_buffer deviceID_priv;
+  //                          loc_buffer cdi;
+  //                          loc_buffer deviceID_label]));
+
+  printf "Deriving DeviceID\n" done;
+  derive_DeviceID
+    (* pub *) deviceID_pub
+    (* priv*) deviceID_priv
+    (* cdi *) cdi
+    (* lbl *) deviceID_label_len
+              deviceID_label;
+
+  (**) let hsd = HST.get () in
+  (**) B.modifies_trans
+          B.loc_none h0 hs1
+         (B.loc_buffer deviceID_pub `B.loc_union` B.loc_buffer deviceID_priv) hsd;
+  // (**) B.modifies_buffer_elim cdi (B.loc_buffer deviceID_pub `B.loc_union` B.loc_buffer deviceID_priv) h0 hsd;
+
+  printf "Deriving AliasKey\n" done;
+  derive_AliasKey
+    (* pub *) aliasKey_pub
+    (* priv*) aliasKey_priv
+    (* cdi *) cdi
+    (* fwid*) fwid
+    (* lbl *) aliasKey_label_len
+              aliasKey_label;
+
+  (**) let hsa = HST.get () in
+  (**) B.modifies_trans
+         (B.loc_buffer deviceID_pub `B.loc_union ` B.loc_buffer deviceID_priv) h0 hsd
+         (B.loc_buffer aliasKey_pub `B.loc_union` B.loc_buffer aliasKey_priv) hsa;
+
+  classify_public_buffer 32ul deviceID_pub deviceID_pub_sec;
+
+  // assert ((B.loc_buffer deviceID_pub `B.loc_union` B.loc_buffer deviceID_priv) `B.loc_union`
+  //                     (B.loc_buffer aliasKey_pub `B.loc_union` B.loc_buffer aliasKey_priv)
+  //         ==
+  //         B.loc_buffer deviceID_pub `B.loc_union` B.loc_buffer deviceID_priv `B.loc_union`
+  //                     B.loc_buffer aliasKey_pub `B.loc_union` B.loc_buffer aliasKey_priv); admit()
+
+  (**) let hsa1 = HST.get () in
+  assert (B.modifies ((B.loc_buffer deviceID_pub `B.loc_union` B.loc_buffer deviceID_priv) `B.loc_union`
+                      (B.loc_buffer aliasKey_pub `B.loc_union` B.loc_buffer aliasKey_priv)) h0 hsa); admit();
+  // (**) B.modifies_trans
+  //        (B.loc_buffer deviceID_pub `B.loc_union` B.loc_buffer deviceID_priv `B.loc_union`
+  //         B.loc_buffer aliasKey_pub `B.loc_union` B.loc_buffer aliasKey_priv) h0 hsa
+  //        (B.loc_buffer deviceID_pub_sec) hsa1;
+  derive_authKeyID
+    aliasKeyCrt_keyID
+    deviceID_pub_sec;
+
+
+  (**) let hsf = HST.get () in
+  // assert (B.modifies (B.loc_buffer deviceID_pub `B.loc_union` B.loc_buffer deviceID_priv) hs0 hsf);
+  HST.pop_frame ();
+  (**) let hf = HST.get () in
+  (**) B.popped_modifies hsf hf;
+  assume (B.modifies (B.loc_all_regions_from false (HS.get_tip hs0) `B.loc_union`
+                      (B.loc_buffer aliasKey_pub `B.loc_union` B.loc_buffer aliasKey_priv)) hs0 hsf);
+  B.modifies_fresh_frame_popped h0 hs0 (B.loc_buffer aliasKey_pub `B.loc_union` B.loc_buffer aliasKey_priv) hsf hf;
+  // assert (B.modifies (B.loc_buffer deviceID_pub `B.loc_union` B.loc_buffer deviceID_priv) hs0 hf);
+  // (**) B.modifies_remove_fresh_frame h0 hs0 hf B.loc_none;
+  (**) assert (B.modifies (B.loc_buffer aliasKey_pub `B.loc_union` B.loc_buffer aliasKey_priv) h0 hf);
+  (**) assume (HST.equal_domains h0 hf)
+
+(*)
+  B.modifies_fresh_frame_popped h0 hs0 B.loc_none hs0 hf;
+  Set.lemma_equal_intro (Map.domain (HS.get_hmap h0)) (Map.domain (HS.get_hmap hf));
+  assert (Set.equal (Map.domain (HS.get_hmap h0)) (Map.domain (HS.get_hmap hf)));
+  // HST.lemma_same_refs_in_all_regions_intro h0 hf;
+  // assert (HST.same_refs_in_all_regions h0 hf);
+  assert (HST.equal_domains h0 hf);
+  admit();
+
+(* Derive DeviceID *)
+  let deviceID_pub : B.lbuffer byte_pub 32 = B.alloca 0x00uy    32ul in
+  let deviceID_priv: B.lbuffer byte_sec 32 = B.alloca (u8 0x00) 32ul in
+
+  let h = HST.get () in
+  // assume (B.(all_live h [buf deviceID_pub;
+  //                        buf deviceID_priv;
+  //                        buf cdi;
+  //                        buf deviceID_label]));
+  // assume (B.(all_disjoint [loc_buffer deviceID_pub;
+  //                          loc_buffer deviceID_priv;
+  //                          loc_buffer cdi;
+  //                          loc_buffer deviceID_label]));
+  printf "Deriving DeviceID\n" done;
+  derive_DeviceID
+    (* pub *) deviceID_pub
+    (* priv*) deviceID_priv
+    (* cdi *) cdi
+    (* lbl *) deviceID_label_len
+              deviceID_label;
+  HST.pop_frame ();
+  // let hf = HST.get () in
+  // assume (HST.equal_domains h0 hf)
+
+(* A workaround to derive authKeyID for now *)
+  let deviceID_pub_sec: B.lbuffer byte_sec 32 = B.alloca (u8 0x00) 32ul in
+  let aliasKeyCrt_keyID: B.lbuffer byte_pub 20 = B.alloca 0x00uy 20ul in
+  classify_public_buffer 32ul deviceID_pub deviceID_pub_sec;
+  derive_authKeyID
+    aliasKeyCrt_keyID
+    deviceID_pub_sec;
+  // let aliasKeyCrt_keyID: datatype_of_asn1_type OCTET_STRING = (|20ul, B32.of_buffer 20ul aliasKeyCrt_keyID_buf|) in
+
+(* Derive AliasKey *)
+  printf "Deriving AliasKey\n" done;
+  derive_AliasKey
+    (* pub *) aliasKey_pub
+    (* priv*) aliasKey_priv
+    (* cdi *) cdi
+    (* fwid*) fwid
+    (* lbl *) aliasKey_label_len
+              aliasKey_label;
+
+  // let h_AliasKey = HST.get () in
+
+  let h2 = HST.get () in
+  // assume (HS.poppable h);
+  HST.pop_frame();
+
+  // B.modifies_fresh_frame_popped
+
+  let h3 = HST.get () in
+  assume (B.modifies B.loc_none h2 h3);
+  // assume (HST.equal_domains h0 h3);
+
+
+(* Create DeviceIDCRI *)
+   let deviceIDCRI_len: asn1_TLV_int32_of_type SEQUENCE = len_of_deviceIDCRI
+                                                            deviceIDCSR_ingredients.deviceIDCSR_version
+                                                            deviceIDCSR_ingredients.deviceIDCSR_s_common
+                                                            deviceIDCSR_ingredients.deviceIDCSR_s_org
+                                                            deviceIDCSR_ingredients.deviceIDCSR_s_country in
+   let deviceIDCRI_buf: B.lbuffer byte_pub (v deviceIDCRI_len) = B.alloca 0x00uy deviceIDCRI_len in
+
+   let h = HST.get () in
+   assume (B.(all_live h [buf deviceID_pub;
+                          buf deviceIDCRI_buf]));
+   assume (B.(all_disjoint [loc_buffer deviceID_pub;
+                            loc_buffer deviceIDCRI_buf]));
+
+   printf "Creating DeviceID Certificate Signing Request Information\n" done;
+   create_deviceIDCRI
+    (* version   *) deviceIDCSR_ingredients.deviceIDCSR_version
+                    deviceIDCSR_ingredients.deviceIDCSR_s_common
+                    deviceIDCSR_ingredients.deviceIDCSR_s_org
+                    deviceIDCSR_ingredients.deviceIDCSR_s_country
+    (* key usage *) deviceIDCSR_ingredients.deviceIDCSR_ku
+    (* DeviceID  *) deviceID_pub
+    (*DeviceIDCRI*) deviceIDCRI_len
+                    deviceIDCRI_buf;
+
+(* Zhe 10/06: Hard to be proved even with 100 more z3rlimits. *)
+  let h = HST.get () in
+  assume (B.(all_live h [buf deviceID_priv;
+                         buf deviceIDCRI_buf;
+                         buf deviceIDCSR_buf]));
+  assume (B.(all_disjoint [loc_buffer deviceID_priv;
+                           loc_buffer deviceIDCRI_buf;
+                           loc_buffer deviceIDCSR_buf]));
+
+  // assume (0 < v deviceIDCRI_len);
+  // assume (valid_deviceIDCSR_ingredients deviceIDCSR_len);
+  // assume (v deviceIDCSR_len == length_of_deviceIDCSR deviceIDCRI_len);
+
+(* Sign AliasKeyTBS and Finalize AliasKeyCRT *)
+  printf "Signing and finalizing DeviceID Certificate Signing Request\n" done;
+  sign_and_finalize_deviceIDCSR
+    (*Signing Key*) deviceID_priv
+    (*DeviceIDCRI*) deviceIDCRI_len
+                    deviceIDCRI_buf
+    (*DeviceIDCSR*) deviceIDCSR_len
+                    deviceIDCSR_buf;
+(* Create AliasKeyTBS *)
+  let aliasKeyTBS_len: asn1_TLV_int32_of_type SEQUENCE = len_of_aliasKeyTBS
+                                                           aliasKeyCRT_ingredients.aliasKeyCrt_serialNumber
+                                                           aliasKeyCRT_ingredients.aliasKeyCrt_i_common
+                                                           aliasKeyCRT_ingredients.aliasKeyCrt_i_org
+                                                           aliasKeyCRT_ingredients.aliasKeyCrt_i_country
+                                                           aliasKeyCRT_ingredients.aliasKeyCrt_s_common
+                                                           aliasKeyCRT_ingredients.aliasKeyCrt_s_org
+                                                           aliasKeyCRT_ingredients.aliasKeyCrt_s_country
+                                                           aliasKeyCRT_ingredients.aliasKeyCrt_riot_version in
+  let aliasKeyTBS_buf: B.lbuffer byte_pub (v aliasKeyTBS_len) = B.alloca 0x00uy aliasKeyTBS_len in
+
+  let h = HST.get () in
+  assume (B.(all_live h [buf fwid;
+                         buf deviceID_pub;
+                         buf aliasKey_pub;
+                         buf aliasKeyCrt_keyID;
+                         buf aliasKeyTBS_buf]));
+
+  assume (B.(all_disjoint [loc_buffer fwid;
+                           loc_buffer deviceID_pub;
+                           loc_buffer aliasKey_pub;
+                           loc_buffer aliasKeyCrt_keyID;
+                           loc_buffer aliasKeyTBS_buf]));
+
+  printf "Creating AliasKey Certificate TBS\n" done;
+  create_aliasKeyTBS
+    (aliasKeyCRT_ingredients.aliasKeyCrt_version)
+    (aliasKeyCRT_ingredients.aliasKeyCrt_serialNumber)
+    (aliasKeyCRT_ingredients.aliasKeyCrt_i_common)
+    (aliasKeyCRT_ingredients.aliasKeyCrt_i_org)
+    (aliasKeyCRT_ingredients.aliasKeyCrt_i_country)
+    (aliasKeyCRT_ingredients.aliasKeyCrt_notBefore)
+    (aliasKeyCRT_ingredients.aliasKeyCrt_notAfter)
+    (aliasKeyCRT_ingredients.aliasKeyCrt_s_common)
+    (aliasKeyCRT_ingredients.aliasKeyCrt_s_org)
+    (aliasKeyCRT_ingredients.aliasKeyCrt_s_country)
+    (fwid)
+    (aliasKeyCRT_ingredients.aliasKeyCrt_ku)
+    (aliasKeyCrt_keyID)
+    (aliasKeyCRT_ingredients.aliasKeyCrt_riot_version)
+    (* DeviceID  *) deviceID_pub
+    (* AliasKey  *) aliasKey_pub
+    (*AliasKeyTBS*) aliasKeyTBS_len
+                    aliasKeyTBS_buf;
+
+  assume (B.(all_live h [buf deviceID_priv;
+                         buf aliasKeyTBS_buf;
+                         buf aliasKeyCRT_buf]));
+  assume (B.(all_disjoint [loc_buffer deviceID_priv;
+                           loc_buffer aliasKeyTBS_buf;
+                           loc_buffer aliasKeyCRT_buf]));
+
+(* Sign AliasKeyTBS and Finalize AliasKeyCRT *)
+  printf "Signing and finalizing AliasKey Certificate\n" done;
+  sign_and_finalize_aliasKeyCRT
+    (*Signing Key*) deviceID_priv
+    (*AliasKeyTBS*) aliasKeyTBS_len
+                    aliasKeyTBS_buf
+    (*AliasKeyCRT*) aliasKeyCRT_len
+                    aliasKeyCRT_buf;
+
+  let h = HST.get () in
+  assume (HS.poppable h);
+  HST.pop_frame();
+
+  let h = HST.get () in
+  assume (HST.equal_domains h0 h);
+  assume (B.(modifies (loc_buffer deviceIDCSR_buf `loc_union`
+                       loc_buffer aliasKeyCRT_buf `loc_union`
+                       loc_buffer aliasKey_pub    `loc_union`
+                       loc_buffer aliasKey_priv ) h0 h) );
+  assume (B.as_seq h_AliasKey aliasKey_pub  == B.as_seq h aliasKey_pub /\
+          B.as_seq h_AliasKey aliasKey_priv == B.as_seq h aliasKey_priv);
+  // assume (aliasKey_post cdi fwid aliasKey_label_len aliasKey_label aliasKey_pub aliasKey_priv h0 h)
+  // assume (riot_post
+  //                       (cdi)
+  //                       (fwid)
+  //                       (deviceID_label_len) (deviceID_label)
+  //                       (aliasKey_label_len) (aliasKey_label)
+  //                       (deviceIDCSR_ingredients)
+  //                       (aliasKeyCRT_ingredients)
+  //                       (aliasKey_pub) (aliasKey_priv)
+  //                       (deviceIDCSR_len) (deviceIDCSR_buf)
+  //                       (aliasKeyCRT_len) (aliasKeyCRT_buf)
+  //                       (h0) (h))
